examples/MemCacheInl.v
@@ -1,0 +1,28 @@
+Require Import Lts.Syntax Lts.Semantics Lts.Equiv Lts.Refinement Lts.Renaming Lts.Wf.
+Require Import Lts.Inline Lts.InlineFacts_2 Lts.Tactics.
+Require Import Ex.SC Ex.MemCache.
+
+Set Implicit Arguments.
+
+Section MemCacheInl.
+  Variables IdxBits TagBits LgNumDatas LgDataBytes: nat.
+  Variable Id: Kind.
+  Variable FifoSize: nat.
+
+  Definition n := 1. (* number of caches (cores) *)
+
+  Definition memCache := memCache IdxBits TagBits LgNumDatas LgDataBytes Id FifoSize n.
+  Hint Unfold memCache: ModuleDefs. (* for kinline_compute *)
+  
+  Definition memCacheInl: Modules * bool.
+  Proof.
+    remember (inlineF memCache) as inlined.
+    kinline_compute_in Heqinlined.
+    match goal with
+    | [H: inlined = ?m |- _] =>
+      exact m
+    end.
+  Defined.
+
+End MemCacheInl.
+
